\documentclass[11pt]{article}
\usepackage{amsthm}
\usepackage{amsmath}

\newcommand{\numpy}{{\tt numpy}}    % tt font for numpy

\topmargin -.5in
\textheight 9in
\oddsidemargin -.25in
\evensidemargin -.25in
\textwidth 7in

\newtheorem{theorem}{Theorem}[section]
\newtheorem{corollary}{Corollary}[theorem]
\newtheorem*{lemma}{Lemma}

\theoremstyle{definition}
\newtheorem*{definition}{Definition}
\begin{document}

% ========== Edit your name here
\author{}
\title{Proof of Pumping Lemma using Regular Expression}
\maketitle

\medskip
\begin{definition}The length of a regular expression is defined as follows: Consider a regular expression $R$.
\begin{itemize}
    \item If $R = a$, where $a$ is a single character, then $|R| = 1$.
    \item If $R = \varepsilon$, then $|R| = 0$. 
    \item If $R = R_1R_2$, the concatenation of regular expressions $R_1$ and $R_2$, then $|R| = |R_1| + |R_2|$.
    \item If $R = R_1^*$, the star of the regular expression $R_1$, then $|R| = |R_1|$. 
    \item If $R = R_1 \cup R_2$, the union of regular expressions $R_1$ and $R_2$, then $|R| = \max(R_1, R_2)$.
\end{itemize}
\end{definition}
\begin{definition}
A regular expression $R$ is a \textbf{reduced regular expression} if $R = A_1B_1^*A_2B_2^*...A_{n-1}B_{n-1}^*A_n$ for which
\begin{enumerate}
    \item $A_i \in \Sigma^*$ for all $i$ (i.e. $A_i$ contains no union or star operation).
    \item $B_i$ is non-empty regular expression for all $i$.
\end{enumerate}
\end{definition}
\begin{lemma}[Pumping Lemma for Reduced Regular Expression] Let $R$ be a reduced regular expression. Then there exists an integer $p\geq 1$ depending only on $R$ such that any string $w \in L(R)$ of length at least $p$ can be written as $w = xyz$, satisfying the following conditions:
\begin{enumerate}
    \item $|y| \geq = 1$
    \item $|xy|\leq p$
    \item $(\forall n\geq 0)(xy^nz\in L(R))$
\end{enumerate}
\end{lemma}
\begin{proof}
Let $p$ be the length of $R$ plus $1$. Take any $w\in L(R)$ with $|w|\geq p$. Since $R$ is a reduced regular expression, $R = A_1B_1^*A_2B_2^*...A_{n-1}B_{n-1}^*A_n$ with $A_i \in \Sigma^*$ and $B_i$ nonempty regular expression. Since $w \in L(R)$, there exists $a_1, a_2, ... ,a_n, b_1, b_2, ...,b_{n-1}$ such that $w = a_1b_1 ... a_{n-1}b_{n-1}a_n$ with $a_i \in L(A_i)$ and $b_i\in L(B_i^*)$ for all $i$.

Since $a_i \in L(A_i)$ and $A_i \in \Sigma^*$, $|a_i| \leq |A_i|$. Then 
\begin{align*}
    |w| &= \sum_{i=1}^n{|a_i|} + \sum_{i=1}^{n-1}{|b_i|}\\
    |w| &\leq \sum_{i=1}^n{|A_i|} + \sum_{i=1}^{n-1}{|b_i|}
\end{align*}

Since $|w| \geq p = |R| + 1$, $\sum_{i=1}^n{|A_i|} \leq |R|$, we must have $\sum_{i=1}^{n-1}{|b_i|} \geq 1$. Hence there exists at least one $k$ such that $|b_k| \geq 1|$. Pick the $b_k$ with the smallest index, such that $|b_i| = 0$ for all $i < k$.

Since $b_k \in L(B_k^*)$, there exists $y\in B_k$ such that $b_k = y^t$ for some $t\geq 1$ and $y^n \in B_k ^*$ for all n. 

Let $x = a_1b_1a_2 ... b_{k-1}a_k$, $z = y^{t-1}a_{k+1}b_{k+1}...b_{n-1}a_n$, then we have
\begin{enumerate}
    \item[-] $|y| \geq = 1$ since $|y^t| \geq 1$.
    \item[-] $|xy|\leq p$ since $|xy| = \sum_{i=1}^{k}|a_i| + \sum_{i=1}^{k-1}|b_i| + |y| \leq \sum_{i=1}^{k}|A_i| + 0 + |B_k| \leq p$
    \item[-] $(\forall n\geq 0)(xy^nz\in L(R))$ since 
    \begin{align*}
        xy^nz &= (a_1b_1a_2 ... b_{k-1}a_k)(y^n)(y^{t-1}a_{k+1}b_{k+1}...b_{n-1}a_n)\\
        &= a_1b_1a_2 ... b_{k-1}a_ky^{n +t-1}a_{k+1}b_{k+1}...b_{n-1}a_n \in L(R)
    \end{align*}
    because $a_i\in A_i$ for all i, $b_i \in B_i^*$ for all $i \neq k$ and $y^{n +t-1} \in B_k$.
\end{enumerate}
Thus proving the pumping lemma.
\end{proof}

\end{document}
\grid
\grid
